strlen example done

c/poc/strlen_spec.v
@@ -5,99 +5,17 @@ From Coq Require Import String List ZArith Psatz.
 From compcert Require Import Coqlib Integers Floats AST Ctypes Cop Clight Clightdefs Memory Values ClightBigstep Events Maps.
 (* Local Open Scope Z_scope.*)
 
-(* Some useful notation and tactics *)
 
-Definition chunk : memory_chunk := Mint8unsigned.
-Definition VintZ := fun (z : Z) => Vint (Int.repr z).
-Definition VintN:= fun n => Vint (Int.repr(Z_of_nat n)).
-Definition VintP := fun p : positive => Vint (Int.repr (Z.pos p)).
+(* Specification of the strlen function *)
 
-Notation gso := PTree.gso.
-Notation gss := PTree.gss.
+Inductive strlen_mem (m : mem) (b : block) (ofs : Z) : nat -> Prop :=
+| LengthZeroMem: Mem.load Mint8unsigned m b ofs = Some (Vint Int.zero) -> strlen_mem m b ofs 0
+| LengthSuccMem: forall n c,
+    strlen_mem m b (ofs+1) n ->
+    Mem.load Mint8unsigned m b ofs = Some (Vint c) ->
+    c <> Int.zero ->
+    strlen_mem m b ofs (S n).
 
-(* Tactics for arithmetic on ptrofs, now they are ad hoc, TODO: automatize translation from ptrofs to Z *)
-
-Ltac ints_to_Z :=
-  repeat rewrite Int.unsigned_repr_eq; repeat rewrite Zmod_small.
-
-Ltac ptrofs_to_Z :=
-  repeat rewrite Ptrofs.unsigned_repr_eq; repeat rewrite Zmod_small.
-
-Ltac ptrofs_compute_add_mul :=
-      simpl; unfold Ptrofs.add; unfold Ptrofs.mul; unfold Ptrofs.of_intu; unfold Ptrofs.of_int;
-      repeat rewrite Ptrofs.unsigned_repr_eq;  repeat rewrite Int.unsigned_repr_eq; repeat rewrite Zmod_small.
-
-Ltac ints_compute_add_mul :=
-      simpl; unfold Int.add; unfold Int.mul;
-      repeat rewrite Int.unsigned_repr_eq;  repeat rewrite Int.unsigned_repr_eq; repeat rewrite Zmod_small.
-
-Ltac seq1 := eapply exec_Sseq_1.
-Ltac seq2 := eapply exec_Sseq_2.
-Ltac sset := eapply exec_Sset.
-Ltac loop := eapply exec_Sloop_loop.
-Ltac gss := eapply gss.
-
-Ltac gso_assumption :=
-  match goal with
-  | [ H : ?P ! ?I = Some ?W |- (PTree.set _ _ ?P) ! ?I = Some ?Z ] => rewrite gso  
-  | [ H : ?P ! ?Q = Some ?W |-  ?P ! ?Q = Some ?Z ] => apply H
-  | [ |- _ <> _ ] => cbv ; congruence
-  end.
-
- Ltac invert_clear :=
-        match goal with
-          | [H : context[exec_stmt] |- _] =>
-            inversion_clear H 
-          | [H : context[eval_expr] |- _] =>
-            inversion_clear H 
-          | [H : context[eval_lvalue] |- _] =>
-            inversion_clear H 
-          | [H : context[bool_val] |- _] =>
-            inversion_clear H  
-          | [H : context[deref_loc] |- _] =>
-            inversion_clear H  
-          | [H : context[sem_binary_operation] |- _] =>
-           inversion_clear H  
-          | [H : context[access_mode] |- _] =>
-            inversion_clear H
-          | [H : context[ out_break_or_return] |- _] => inversion_clear H                  
-          | _ => idtac
-        end.    
-
-
-Ltac solve_by_inverts n :=
-   match n with
-   | O => idtac
-   | S (?n') => invert_clear ; solve_by_inverts n'
-end.
-
-(* Recursive specification of strlen function *)
-
-(* unsigned C char *)
-Definition C_uchar : Set := positive.
-
- (* C string *) 
-Inductive C_string : Set :=
-| CEmptyString : C_string
-| CString : positive -> C_string -> C_string.
-
-Inductive strlen : C_string -> nat -> Prop :=
-| LengthZero : strlen CEmptyString 0
-| LengthSucc : forall n s c, strlen s n -> strlen (CString c s) (S n).
-
-Inductive strlen_mem_op : mem -> block -> Z -> option (C_string*nat) -> Prop :=
-| LengthZeroMem_op : forall m b ofs, Mem.load Mint8signed m b ofs = Some (VintZ 0) -> strlen_mem_op m b ofs (Some (CEmptyString, O))
-| LengthSuccMem_op : forall m b ofs c s n, strlen_mem_op m b (ofs + 1) (Some (s,n)) -> Mem.load Mint8signed m b ofs = Some (VintP c) -> strlen_mem_op m b ofs (Some ((CString c s),(S n))).
-
-Inductive strlen_mem : mem -> block -> Z -> nat -> Prop :=
-| LengthZeroMem m b ofs: Mem.load Mint8unsigned m b ofs = Some (VintZ 0) -> strlen_mem m b ofs 0
-| LengthSuccMem m b ofs: forall p v,
-    strlen_mem m b (ofs+1) p ->
-    Mem.load Mint8unsigned m b ofs = Some (VintP v) ->
-    strlen_mem m b ofs (S p).
-
-
-(* Try induction on strlen type *)
 
 (* strlen C light AST *)
 
@@ -151,7 +69,6 @@ Definition f_strlen_loop :=
             tuint)))
       Sskip).
 
-Print Sloop.
 
 Definition f_strlen_loop_body := (Ssequence
         (Ssequence
@@ -165,176 +82,51 @@ Definition f_strlen_loop_body := (Ssequence
             (Sifthenelse (Etempvar _t'2 tuchar) Sskip Sbreak)))
         (Sset _output
           (Ebinop Oadd (Etempvar _output tuint) (Econst_int (Int.repr 1) tint)
-            tuint))).
+                  tuint))).
 
-(* Correctness statements *)
-(* On empty string C light function evaluates to 0 *)
+(* Our goal is to prove that the C light AST is equivalent satisfies the spec: in this context it means that the C light AST evaluates to the correct value wrt to big step operational semantics *)
 
-Lemma strlen_correct_loop_empty_string :
-  (* with this assumption Ptrofs.modulus = Int.modulus, ptherwise Ptrofs.modulus > Int.modulus *)
-  Archi.ptr64 = false ->
-  forall ge e m b ofs le len,                       
-    (* Preconditions on the length of the string and valid offset *)
-    0 <= ofs < Ptrofs.modulus ->
-    Z_of_nat len < Int.modulus ->
-    ofs + Z_of_nat len < Ptrofs.modulus ->                      
-    (* Initialize local variables *)
-    le!_input = Some (Vptr b (Ptrofs.repr ofs)) ->
-    le!_output = Some (VintN O) ->                     
-    (* Precondition: reading empty C string from memory *)
-    strlen_mem m b ofs O ->
-    (* C light expression f_strlen returns O and assigns O to output variable *)
-    exists t le', exec_stmt ge e le m f_strlen_loop t le' m Out_normal /\ le'!_output = Some (VintN O).
-Proof.
-  intros.
-  inversion_clear H5.
-  repeat eexists.
-  eapply exec_Sloop_stop1.
-  seq2. repeat econstructor. gso_assumption. apply gss.
-  repeat econstructor. rewrite gso. apply gss. cbv; congruence. simpl.
-  replace (Ptrofs.unsigned (Ptrofs.repr ofs)) with ofs. 
-  apply H6.
-  { pose (Ptrofs.modulus_eq32 H). ptrofs_compute_add_mul. all: nia. }
-  apply gss. econstructor.
-  replace (negb (Int.eq (Int.repr 0) Int.zero)) with false by simpl.
-  econstructor.
-  cbv; congruence.
-  econstructor.
-  repeat (rewrite gso). assumption. all: cbv; congruence.
-Qed.
+(* Some useful notation and tactics *)
 
+Definition chunk : memory_chunk := Mint8unsigned.
+Definition VintZ := fun (z : Z) => Vint (Int.repr z).
+Definition VintN:= fun n => Vint (Int.repr(Z_of_nat n)).
 
-(* Test case: On a string of length 2 C light function evaluates to 0 *)
-Lemma strlen_correct_test :
-  (* with this assumption Ptrofs.modulus = Int.modulus, ptherwise Ptrofs.modulus > Int.modulus *)
-  Archi.ptr64 = false ->
-  forall ge e m b ofs le len,                       
-    (* Preconditions on the length of the string and valid offset *)
-    0 <= ofs < Ptrofs.modulus ->
-    Z_of_nat len < Int.modulus ->
-    ofs + Z_of_nat len < Ptrofs.modulus ->                      
-    (* Initialize local variables *)
-    le!_input = Some (Vptr b (Ptrofs.repr ofs)) ->
-    le!_output = Some (VintZ 0) ->                     
-    (* Precondition: reading  C string of length 2 from memory *)
-    strlen_mem m b ofs 2%nat ->
-    
-    (* C light expression f_strlen returns O and assigns O to output variable *)
-    exists t le', exec_stmt ge e le m f_strlen.(fn_body) t le' m (Out_return (Some ((VintZ 2),tuint))) /\ (le'!_output) = Some (VintZ 2).
-Proof.
-  intros.
-  inversion_clear H5. inversion_clear H6. inversion_clear H5.
-  repeat eexists.
-  - seq1.
-    -- sset. (* evaluate expression *) repeat econstructor.
-    -- seq1.   
-      * (* loop 1 *)
-        loop. repeat econstructor. repeat gso_assumption. eapply gss. repeat econstructor.
-        rewrite gso. apply gss. cbv. congruence. simpl. ptrofs_to_Z. apply H7. assumption.
-        apply gss.
-        simpl.
-        econstructor.
-        replace (negb (Int.eq (Int.repr (Z.pos v)) Int.zero)) with true by admit.      
-        econstructor.
-        repeat econstructor. repeat econstructor. repeat econstructor.
-        rewrite gso. rewrite gso. rewrite gso. apply gss. 1-3: cbv ;congruence.
-        repeat econstructor. econstructor. econstructor.
+Notation gso := PTree.gso.
+Notation gss := PTree.gss.
 
-        (* loop 2 *)
-        loop. repeat econstructor. repeat gso_assumption.
-        rewrite gso. rewrite gso. apply gss. 1-2: cbv ; congruence.
-        apply gss.
-        repeat econstructor.
-        rewrite gso. apply gss. cbv ; congruence.
-        simpl.
-        replace (Ptrofs.unsigned
-                   (Ptrofs.add (Ptrofs.repr ofs) (Ptrofs.mul (Ptrofs.repr 1) (Ptrofs.of_ints (Int.repr 1))))) with (ofs + 1) by admit.
-        apply H8.        
-        apply gss.
-        simpl.
-        econstructor.
-        replace (negb (Int.eq (Int.repr (Z.pos v0)) Int.zero)) with true by admit.      
-        econstructor.
-        rewrite gso. rewrite gso. rewrite gso. apply gss. 1-3: cbv ; congruence.
-        repeat econstructor. econstructor. econstructor.
-            
-         (* exit loop *)
-        eapply exec_Sloop_stop1.
-        seq2. seq1. seq1. econstructor. econstructor. rewrite gso. rewrite gso. apply gss. 1-2: cbv ; congruence.
-        repeat econstructor.
-        apply gss.
-        repeat econstructor.
-        seq1. repeat econstructor.
-        rewrite gso. apply gss. cbv ; congruence.
-        simpl.
-      
-        replace (Ptrofs.unsigned
-       (Ptrofs.add
-          (Ptrofs.add (Ptrofs.repr ofs)
-             (Ptrofs.mul (Ptrofs.repr 1) (Ptrofs.of_ints (Int.repr 1))))
-          (Ptrofs.mul (Ptrofs.repr 1) (Ptrofs.of_ints (Int.repr 1))))) with (ofs + 1 + 1) by admit.        apply H6.
-        repeat econstructor.
-        apply gss.
-        simpl.
-        econstructor. 
-        replace (negb (Int.eq (Int.repr 0) Int.zero)) with false by (simpl).
-        econstructor.
-        cbv; congruence.
-        econstructor.
-      * (* return statement *)
-        repeat econstructor.  rewrite gso.  rewrite gso.  rewrite gso.  eapply gss. all: cbv; congruence.
-  - rewrite gso.  rewrite gso.  rewrite gso.  eapply gss. all: cbv ; congruence.
-Admitted.
+(* Tactics for arithmetic on ptrofs, now they are ad hoc, TODO: automatize translation from ptrofs to Z *)
 
-(* Conditions about the f_strlen loop *)
-(* If 0 is read from memory at [b,ofs + len] the output is set to len *)
-Lemma strlen_loop_break_correct : Archi.ptr64 = false -> forall ge e m b ofs outp le,
-      
-      ofs + Z.of_nat outp < Ptrofs.modulus ->
-      0 <= ofs < Ptrofs.modulus ->
-      0 <= Z.of_nat outp < Ptrofs.modulus ->
+Ltac ints_to_Z :=
+  repeat rewrite Int.unsigned_repr_eq; repeat rewrite Zmod_small.
 
-      (* IF before the loop *s = [b,ofs + outp] and i = outp *)
-      le!_input = Some (Vptr b (Ptrofs.repr (ofs + Z.of_nat outp))) ->
-      le!_output = Some (VintN outp) ->
-      
-      (* and the guard condition is false *)
-      Mem.load Mint8unsigned m b (ofs + (Z_of_nat outp)) = Some (Vint (Int.repr 0)) ->
+Ltac ptrofs_to_Z :=
+  repeat rewrite Ptrofs.unsigned_repr_eq; repeat rewrite Zmod_small.
 
-      (* THEN loop executes to an environment with i = outp [i.e., i stays unchanged] + memory is unchanged *)
-      exists t le', exec_stmt ge e le m f_strlen_loop t le' m Out_normal /\ (le'!_output) = Some (VintN outp).
-Proof.
-  intros.
-  repeat eexists.
-  eapply exec_Sloop_stop1.
-  seq2. seq1. seq1.
-  repeat econstructor.
-  apply H3.
-  repeat econstructor.
-  apply gss.
-  repeat econstructor.
-  seq1.
-  repeat econstructor.
-  rewrite gso. apply gss. cbv ; congruence.
-  unfold Mem.loadv.
-  replace (Ptrofs.unsigned (Ptrofs.repr (ofs + Z.of_nat outp))) with (ofs + Z.of_nat outp) by admit.
-  apply H5.
-  repeat econstructor.
-  apply gss.
-  econstructor.
-  replace (negb (Int.eq (Int.repr 0) Int.zero)) with false by (simpl).
-  econstructor.
-  cbv; congruence.
-  econstructor.
-  repeat (rewrite gso). assumption.
-  all: cbv; congruence.
-Admitted.
+Ltac ptrofs_compute_add_mul :=
+      simpl; unfold Ptrofs.add; unfold Ptrofs.mul; unfold Ptrofs.of_intu; unfold Ptrofs.of_int;
+      repeat rewrite Ptrofs.unsigned_repr_eq;  repeat rewrite Int.unsigned_repr_eq; repeat rewrite Zmod_small.
 
-Print exec_stmt.
+Ltac ints_compute_add_mul :=
+      simpl; unfold Int.add; unfold Int.mul;
+      repeat rewrite Int.unsigned_repr_eq;  repeat rewrite Int.unsigned_repr_eq; repeat rewrite Zmod_small.
 
-(* Helper lemmas about strlen_mem *)
+Ltac seq1 := eapply exec_Sseq_1.
+Ltac seq2 := eapply exec_Sseq_2.
+Ltac sset := eapply exec_Sset.
+Ltac loop := eapply exec_Sloop_loop.
 
-Lemma strlen_trans_len_0 : forall len m b ofs, strlen_mem m b ofs len -> strlen_mem m b (ofs + Z.of_nat len) O.
+(* can make more generic to repeatedly apply gso *)
+Ltac gso_assumption :=
+  match goal with
+  | [ H : ?P ! ?I = Some ?W |- (PTree.set _ _ ?P) ! ?I = Some ?Z ] => rewrite gso  
+  | [ H : ?P ! ?Q = Some ?W |-  ?P ! ?Q = Some ?Z ] => apply H
+  | [ |- _ <> _ ] => cbv ; congruence
+  end.
+
+(* Helper lemmas about the specification *)
+
+Lemma strlen_to_len_0 : forall len m b ofs, strlen_mem m b ofs len -> strlen_mem m b (ofs + Z.of_nat len) O.
 Proof.
   induction len ; intros.
   - replace (ofs + Z.of_nat 0) with ofs by nia. assumption.
@@ -343,123 +135,62 @@ Proof.
     apply (IHlen m b (ofs + 1) H0).
 Qed.
 
-Lemma strlen_trans_len_i : forall len m b ofs, strlen_mem m b ofs len -> forall i, (i < len)%nat -> strlen_mem m b (ofs + Z.of_nat i) (len - i)%nat.
-Proof.
-  induction len.
-  - intros. omega.
-  - induction i ; intro.
-    + replace (ofs + Z.of_nat 0) with ofs by nia.
-       replace  (S len - 0)%nat with (S len)%nat by omega. assumption. 
-    + inversion_clear H.
-       assert (i < len)%nat by omega. pose (IHlen m b (ofs + 1) H1 i H).
-       replace (S len - S i)%nat with (len - i)%nat by omega.
-       replace (ofs + Z.of_nat (S i)) with  (ofs + 1 + Z.of_nat i) by nia.
-       assumption.
-Qed.  
-   
 Lemma strlen_to_mem : forall len m b ofs, strlen_mem m b ofs len ->
-                                     forall i, (i < len)%nat -> exists p : positive, Mem.load chunk m b (ofs + Z.of_nat i) = Some (VintP p).
+                                     forall i, (i < len)%nat -> exists c, Mem.load chunk m b (ofs + Z.of_nat i) = Some (Vint c) /\ c <> Int.zero.
 Proof.
   induction len.
   - intros. omega.
   -  induction i ; intro ; inversion_clear H.
     +  replace (ofs + Z.of_nat 0) with ofs by nia.
-       exists v. assumption.
+       exists c. exact (conj H2 H3).
     +  assert (i < len)%nat by omega. pose (IHlen m b (ofs + 1) H1 i H).
        replace (ofs + Z.of_nat (S i)) with  (ofs + 1 + Z.of_nat i) by nia.
        assumption.  
 Qed.
 
-Lemma strlen_loop_body_correct: Archi.ptr64 = false -> forall len ge e m b ofs le,
-      0 <= ofs < Ptrofs.modulus ->
-      Z_of_nat len < Int.modulus ->
-      ofs + Z_of_nat len < Ptrofs.modulus ->
-                       
-      le!_input = Some (Vptr b (Ptrofs.repr (ofs + Z.of_nat len))) ->
-      le!_output = Some (VintN len) ->
-    
-      (exists p, Mem.load chunk m b (ofs + Z.of_nat len) = Some (VintP p)) ->
-                                         
-      exists t le', exec_stmt ge e le m f_strlen_loop_body t le' m Out_normal /\ le'!_output = Some (VintN (S len)).
-Proof.
-  intros.
-  destruct H5 as [p].
-  repeat eexists.
-  repeat seq1.
-  repeat econstructor. apply H3. repeat econstructor.
-  apply gss.
-  repeat econstructor.
-  repeat econstructor.
-  rewrite gso. apply gss. cbv; congruence.
-  simpl.
-  replace (Ptrofs.unsigned (Ptrofs.repr (ofs + Z.of_nat len))) with (ofs + Z.of_nat len) by admit.
-  apply H5.
-  repeat econstructor.
-  apply gss.
-  econstructor.
-  replace (negb (Int.eq (Int.repr (Z.pos p)) Int.zero)) with true by admit.
-  repeat econstructor.
-  repeat econstructor.
-  repeat (rewrite gso).
-  apply H4. 1-3: cbv; congruence.
-  repeat econstructor.
-  unfold VintN.
-  replace (Int.add (Int.repr (Z.of_nat len)) (Int.repr 1)) with (Int.repr (Z.of_nat (S len))) by admit.
-  apply gss.
-Admitted.
+(* Correctness statements *)
 
-
-Lemma exec_succ_output : forall ge e le m b ofs n,
-    (exists t1 le1, exec_stmt ge e (PTree.set _output (VintZ 0) (PTree.set _input (Vptr b (Ptrofs.repr ofs)) le)) m f_strlen_loop t1  (PTree.set _output (VintN n) le1) m Out_normal) ->
-
-    exists t2 le2, exec_stmt ge e (PTree.set _output (VintZ 1) (PTree.set _input (Vptr b (Ptrofs.repr ofs)) le)) m f_strlen_loop t2 (PTree.set _output (VintN (S n)) le2) m Out_normal.
-Admitted.
-
-Lemma exec_succ_output_gen : forall ge e le m b ofs i n,
-    
-    (exists t1 le1, exec_stmt ge e (PTree.set _output (VintN i) (PTree.set _input (Vptr b (Ptrofs.repr (ofs + Z.of_nat i))) le)) m f_strlen_loop t1 (PTree.set _output (VintN n) le1) m Out_normal) ->
-
-
-    (exists t2 le2, exec_stmt ge e  (PTree.set _input (Vptr b (Ptrofs.repr (ofs))) le) m f_strlen_loop t2
-       (PTree.set _output (VintN (n + i)%nat) (PTree.set _input (Vptr b (Ptrofs.repr (ofs))) le2)) m
-       Out_normal).
-  Admitted.
-
-
-Lemma strlen_loop_correct_gen_new : (* with this assumption Ptrofs.modulus = Int.modulus, ptherwise Ptrofs.modulus > Int.modulus *)
-  Archi.ptr64 = false -> (* TODO: remove this assumption *)
+(* A generalization of loop correctness *)
+Lemma strlen_loop_correct_gen :
   forall len i ge e m b ofs le,
-                       
-    (* Preconditions on the length of the string and valid offset *) 0 <= ofs < Ptrofs.modulus ->
-    0 <= ofs + Z_of_nat len + Z_of_nat i < Ptrofs.modulus ->   
-       (* Precondition: reading C string of length len from memory *)
+    (* IF ofs is a valid offset *)
+    0 <= ofs < Ptrofs.modulus ->
+    (* we never surpass the offset limit *)
+    0 <= ofs + Z_of_nat len + Z_of_nat i < Ptrofs.modulus ->
+    (* len and i are within integer bound *)                     
+    Z.of_nat (len + i) < Int.modulus ->
+    
+    (* we read a C string of length len + i from memory*)
     strlen_mem m b ofs (len + i) ->
-              
+    
+    (* THEN there is a trace t and local environment le' such that: *)
     exists t le',
+      (* if output equals i in the starting local environment le *)
       le!_output = Some (VintN i) ->
-      le!_input = Some (Vptr b (Ptrofs.repr (ofs + Z.of_nat i))) ->
+      (* if input is an address [b,ofs + i] in the starting local environment *)
+      le!_input = Some (Vptr b (Ptrofs.repr (ofs + Z.of_nat i))) ->     (* then loop of strlen function executes to le' with output assigned len + i *)
       exec_stmt ge e le m f_strlen_loop t le' m Out_normal /\ le'!_output = Some (VintN (len + i)).
 Proof.
-  induction len; intros until le; intros Bound1 Bound2 Spec; pose (Ptrofs.modulus_eq32 H).
+  induction len; intros until le; intros Bound1 Bound2 Bound3 Spec. (*; pose (Ptrofs.modulus_eq32 H). *)
   - (* Base case *)    
     simpl in Spec.
     repeat eexists.
     (* Exit the loop *)
     eapply exec_Sloop_stop1. seq2. repeat econstructor.
-    apply H1.
+    apply H0.
     eapply gss.
     repeat econstructor.
     rewrite gso. apply gss. cbv. congruence.
     (* Derive memory assumptions from the specification *)
-    pose (Spec_mem := strlen_trans_len_0 i m b ofs Spec).
+    pose (Spec_mem := strlen_to_len_0 i m b ofs Spec).
     inversion_clear Spec_mem.
     simpl. 
-    ptrofs_to_Z. apply H2.
+    ptrofs_to_Z. apply H1.
     lia.
     apply gss.
     simpl.
     econstructor.
-    replace (negb (Int.eq (Int.repr 0) Int.zero)) with false by simpl.      
+    replace (negb (Int.eq Int.zero Int.zero)) with false by (auto with ints).      
     econstructor.
     cbv; congruence. econstructor.
     repeat (rewrite gso).
@@ -467,12 +198,12 @@ Proof.
     assumption.
     1-3: cbv; congruence.
   - (* Ind. Step *)
-    assert (exists char, Mem.load Mint8unsigned m b (ofs + Z.of_nat i) = Some (VintP char)) as Mem. (* maybe not positive char ? *)
+    assert (exists char, Mem.load Mint8unsigned m b (ofs + Z.of_nat i) = Some (Vint char) /\ char <> Int.zero) as Mem. 
     { refine (strlen_to_mem (S len + i) m b ofs Spec i _). omega. }
     destruct Mem as [char Mem].
     (* apply I.H. to le' after one step when starting with i and [b,ofs + i]  *)
     pose (le'' :=  (PTree.set _output (VintN (S i))
-       (PTree.set _t'2 (VintP char) (PTree.set _input
+       (PTree.set _t'2 (Vint char) (PTree.set _input
                (Vptr b (Ptrofs.repr (ofs + Z.of_nat (S i))))
           (PTree.set _t'1
                 (Vptr b (Ptrofs.repr (ofs + Z.of_nat i)))
@@ -485,14 +216,14 @@ Proof.
          Out_normal /\
        le' ! _output = Some (VintN (len + S i))) as Step.
     { eapply IH.
-      1-2: lia.
+      1-3: lia.
       replace (len + S i)%nat with (S len + i)%nat by omega.
       assumption. }
     destruct Step as [s Step]. destruct Step as [t Step].
     (* Do one loop on the goal: then apply IH *)
     repeat eexists.
     loop. repeat econstructor.
-    apply H1.
+    apply H0.
     eapply gss. 
     repeat econstructor.
     rewrite gso. apply gss. cbv; congruence.
@@ -501,27 +232,19 @@ Proof.
     lia.
     apply gss.
     econstructor.
-    replace (negb (Int.eq (Int.repr (Z.pos char)) Int.zero)) with true. (* add lemma or revisit pos p : maybe just non-zero integer: use dependent type *)
+    replace (negb (Int.eq char Int.zero)) with true. (* add lemma or revisit pos p : maybe just non-zero integer: use dependent type *)
     econstructor.
-  {
-    assert ((Int.eq (Int.repr (Z.pos char)) Int.zero = false)).
+  { replace (Int.eq char Int.zero) with false.
+    auto.
     rewrite Int.eq_false.
     reflexivity.
-    unfold Int.zero.
-    assert (0 <> Z.pos char) by lia.
-    pose (Int.eqm_samerepr (Z.pos char) 0).
-    unfold not.
-    intro.
-    pose (Int.eqm_small_eq (Z.pos char) 0).
-    SearchAbout Int.zero.
-    
-    admit. admit. } 
-  repeat (rewrite gso). apply H0. 1-3: cbv; congruence.
+    destruct Mem. assumption. }  
+  repeat (rewrite gso). apply H. 1-3: cbv; congruence.
   repeat econstructor. econstructor. econstructor.
   fold f_strlen_loop.
   replace  (PTree.set _output
        (Vint (Int.add (Int.repr (Z.of_nat i)) (Int.repr 1)))
-       (PTree.set _t'2 (VintP char)
+       (PTree.set _t'2 (Vint char)
           (PTree.set _input
              (Vptr b
                 (Ptrofs.add (Ptrofs.repr (ofs + Z.of_nat i))
@@ -529,9 +252,7 @@ Proof.
                       (Ptrofs.repr (sizeof ge tuchar))
                       (ptrofs_of_int Signed (Int.repr 1)))))
              (PTree.set _t'1
-                (Vptr b (Ptrofs.repr (ofs + Z.of_nat i)))
-             
-                      le)))) with le''.
+                (Vptr b (Ptrofs.repr (ofs + Z.of_nat i))) le)))) with le''.
   eapply Step.
   apply gss.
   unfold le''. rewrite gso. rewrite gso. apply gss.
@@ -554,171 +275,41 @@ Proof.
     f_equal.
     ints_compute_add_mul.
     f_equal.
-    1-3: lia. }
+    all: lia. }
   destruct Step.
   apply gss.
   unfold le''. rewrite gso. rewrite gso. apply gss.
   1-2: cbv; congruence.
   replace (S len + i)%nat with (len + S i)%nat by omega.
   assumption.
-      
-Admitted.
+Qed.      
 
-Lemma strlen_loop_correct_gen : (* with this assumption Ptrofs.modulus = Int.modulus, ptherwise Ptrofs.modulus > Int.modulus *)
-  Archi.ptr64 = false -> (* TODO: remove this assumption *)
-  forall len i ge e m b ofs le,
-                       
-    (* Preconditions on the length of the string and valid offset *)
-    0 <= ofs + Z_of_nat len + Z_of_nat i < Ptrofs.modulus ->   
-                       
-       (* Precondition: reading C string of length len from memory *)
-    strlen_mem m b ofs (len + i) ->
-              
-    exists t le', 
-      exec_stmt ge e (PTree.set _output (VintN i) (PTree.set _input (Vptr b (Ptrofs.repr (ofs + Z.of_nat i)))  le)) m f_strlen_loop t le' m Out_normal /\ le'!_output = Some (VintN (len + i)).
+(* On empty string C light function evaluates to 0 *)
+
+Lemma strlen_correct_loop_empty_string :
+  forall ge e m b ofs le len,                       
+
+    0 <= ofs < Ptrofs.modulus ->
+    Z_of_nat len < Int.modulus ->
+    ofs + Z_of_nat len < Ptrofs.modulus ->                      
+ 
+    strlen_mem m b ofs O ->
+
+    exists t le',
+      le!_output = Some (VintN O) ->
+      le!_input = Some (Vptr b (Ptrofs.repr ofs)) ->
+      exec_stmt ge e le m f_strlen_loop t le' m Out_normal /\ le'!_output = Some (VintN O).
 Proof.
-  induction len.
-  intros until le.
-  intro L.
   intros.
-  repeat eexists.
-   eapply exec_Sloop_stop1.
-   seq2. seq1. seq1. repeat econstructor. rewrite gso. eapply gss. cbv; congruence.
-   repeat econstructor.
-   apply gss. repeat econstructor.
-   repeat econstructor.
-  rewrite gso. apply gss. cbv. congruence.
-  simpl in H5.
-  pose (S := strlen_trans_len_0 i m b ofs H5).
-  inversion_clear S.
-  simpl. 
+  replace O with (0 + 0)%nat by lia.
+  replace ofs with (ofs + 0) by lia.
+  eapply strlen_loop_correct_gen.
+  1-3: lia.
+  simpl. assumption.
+Qed.    
 
-  ptrofs_to_Z. apply H6. lia.
-  apply gss.
-  simpl.
-  econstructor.
-  replace (negb (Int.eq (Int.repr 0) Int.zero)) with false by simpl.      
-  econstructor.
-  cbv; congruence. econstructor.
-  rewrite gso. rewrite gso. rewrite gso. replace (0 + i)%nat with i by lia. apply gss. 1-3: cbv; congruence.
-  intros.
-  assert (exists p, Mem.load Mint8unsigned m b (ofs + Z.of_nat i) = Some (VintP p)) as M.
-  { refine (strlen_to_mem (S len + i) m b ofs H6 i _).
-  omega. } 
-  (* follows from spec H5 *)
-  destruct M as [p M].
-  pose (IH := IHlen (S i) ge e m b ofs (
-       (PTree.set _t'2 (VintP p)
-          (
-             (PTree.set _t'1
-                (Vptr b (Ptrofs.repr (ofs + Z.of_nat i)))
-                (PTree.set _output (VintN i)
-                   (PTree.set _input
-                      (Vptr b (Ptrofs.repr (ofs + Z.of_nat i)))
-                      le))))))).
-  
-  assert ( exists (t : trace) (le' : temp_env),
-       exec_stmt ge e
-         (PTree.set _output (VintN (S i))
-            (PTree.set _input
-               (Vptr b (Ptrofs.repr (ofs + Z.of_nat (S i))))
-               (PTree.set _t'2 (VintP p)
-                  (PTree.set _t'1
-                     (Vptr b (Ptrofs.repr (ofs + Z.of_nat i)))
-                     (PTree.set _output (VintN i)
-                        (PTree.set _input
-                           (Vptr b
-                              (Ptrofs.repr (ofs + Z.of_nat i)))
-                           le)))))) m f_strlen_loop t le' m
-         Out_normal /\
-       le' ! _output = Some (VintN (len + S i)) ) as Step.
-  { pose (Ptrofs.modulus_eq32 H).
-  eapply IH.
-  1-6: lia.
-  replace (len + S i)%nat with (S len + i)%nat by omega.
-  assumption. }
-
-  destruct Step as [s St]. destruct St as [t St]. destruct St as [St C].     
-  (* do one loop *)
-  repeat eexists.
-  loop. repeat econstructor.
-  rewrite gso.
-  eapply gss. cbv ; congruence.
-  apply gss.
-  repeat econstructor.
-  rewrite gso. apply gss. cbv. congruence. simpl. ptrofs_to_Z.
-  
-  apply M. lia.
-  apply gss.
-  econstructor.
-  replace (negb (Int.eq (Int.repr (Z.pos p)) Int.zero)) with true. (* add lemma *)
-  econstructor.
-  {
-    assert ( (Int.eq (Int.repr (Z.pos p)) Int.zero) = false).
-    rewrite Int.eq_false.
-    reflexivity.
-    unfold Int.zero.
-    assert (0 <> Z.pos p) by lia.
-    
-    pose (Int.eqm_samerepr (Z.pos p) 0).
-    unfold not.
-    intro.
-    pose (Int.eqm_small_eq (Z.pos p) 0).
-    unfold not in H7.
-
-    SearchAbout Int.zero.
-    
-    admit.
-     }
-  rewrite gso. rewrite gso. rewrite gso. apply gss. 1-3: cbv ;congruence.
-  repeat econstructor. econstructor. econstructor.
-  fold f_strlen_loop.
-  replace  (PTree.set _output
-       (Vint (Int.add (Int.repr (Z.of_nat i)) (Int.repr 1)))
-       (PTree.set _t'2 (VintP p)
-          (PTree.set _input
-             (Vptr b
-                (Ptrofs.add (Ptrofs.repr (ofs + Z.of_nat i))
-                   (Ptrofs.mul
-                      (Ptrofs.repr (sizeof ge tuchar))
-                      (ptrofs_of_int Signed (Int.repr 1)))))
-             (PTree.set _t'1
-                (Vptr b (Ptrofs.repr (ofs + Z.of_nat i)))
-                (PTree.set _output (VintN i)
-                   (PTree.set _input
-                      (Vptr b (Ptrofs.repr (ofs + Z.of_nat i)))
-                      le)))))) with (PTree.set _output (VintN (S i))
-            (PTree.set _input
-               (Vptr b (Ptrofs.repr (ofs + Z.of_nat (S i))))
-               (PTree.set _t'2 (VintP p)
-                  (PTree.set _t'1
-                     (Vptr b (Ptrofs.repr (ofs + Z.of_nat i)))
-                     (PTree.set _output (VintN i)
-                        (PTree.set _input
-                           (Vptr b
-                              (Ptrofs.repr (ofs + Z.of_nat i)))
-                           le)))))).
-  
-  eapply St.
-
-  {
-    replace (Vint (Int.add (Int.repr (Z.of_nat i)) (Int.repr 1))) with (VintN (S i)) by admit.
-    replace (Ptrofs.add (Ptrofs.repr (ofs + Z.of_nat i))
-                (Ptrofs.mul (Ptrofs.repr (sizeof ge tuchar))
-                            (ptrofs_of_int Signed (Int.repr 1)))) with
-        (Ptrofs.repr (ofs + Z.of_nat (S i))) by admit.
-
-    
-    admit.
-  }
-
-  replace (S len + i)%nat with (len + S i)%nat by omega.
-  assumption.
-      
-Admitted.
-
+(* Correctness of the loop execution *)
 Lemma strlen_loop_correct :
-   Archi.ptr64 = false ->
    forall len ge e m b ofs le,
      
     0 <= ofs < Ptrofs.modulus ->
@@ -727,39 +318,243 @@ Lemma strlen_loop_correct :
                        
     strlen_mem m b ofs len ->
               
-    exists t le', exec_stmt ge e (PTree.set _output (VintN O) (PTree.set _input (Vptr b (Ptrofs.repr ofs)) le)) m f_strlen_loop t le' m Out_normal /\ le'!_output = Some (VintN len).
+    exists t le',
+      
+      le!_output = Some (VintN O) ->
+      le!_input = Some (Vptr b (Ptrofs.repr ofs)) ->
+      
+      exec_stmt ge e le m f_strlen_loop t le' m Out_normal /\ le'!_output = Some (VintN len).
 Proof.
   intros.
-  Check strlen_loop_correct.
   replace ofs with (ofs + Z.of_nat O) by lia.
   replace len with (len + O)%nat by lia.
-  eapply (strlen_loop_correct H len O ge e m b ofs le).
-  1-6: lia.
+  eapply strlen_loop_correct_gen.
+  1-3: lia. 
   replace (len + O)%nat with len by omega.
   assumption.
 Qed.
   
 (* Full correctness statement *)
-Lemma strlen_correct : (* with this assumption Ptrofs.modulus = Int.modulus, ptherwise Ptrofs.modulus > Int.modulus *)
-  Archi.ptr64 = false ->
-  
-  forall len ge e m b ofs le,
-                       
-    (* Preconditions on the length of the string and valid offset *)
-    0 < ofs < Ptrofs.modulus ->
+Lemma strlen_correct :  forall len ge e m b ofs le,
+
+    0 <= ofs < Ptrofs.modulus ->
     Z_of_nat len < Int.modulus ->
     ofs + Z_of_nat len < Ptrofs.modulus ->
                        
-                       (* Initialize local variables *)
-    le!_input = Some (Vptr b (Ptrofs.repr ofs)) ->
-    le!_output = Some (VintZ 0) ->
-                       
-       (* Precondition: reading C string of length len from memory *)
     strlen_mem m b ofs len ->
                
-      exists t le', exec_stmt ge e le m f_strlen.(fn_body) t le' m (Out_return (Some ((VintN len),tuint))).
+    exists t le',
+      
+      le!_input = Some (Vptr b (Ptrofs.repr ofs)) ->
+      le!_output = Some (VintZ 0) ->
+      
+      exec_stmt ge e le  m f_strlen.(fn_body) t le' m (Out_return (Some ((VintN len),tuint))).
 Proof.
-  (* follows from strlen_loop_correct *)
-   Admitted.
+  intros.
+  pose (Loop := strlen_loop_correct len ge e  _ _ _ (PTree.set _output (Vint Int.zero) le) H H0 H1 H2). destruct Loop as [t Loop]. destruct Loop as [le' Loop].
+  repeat eexists.
+  intro input.
+  intro output.
+  assert ((PTree.set _output (Vint Int.zero) le) ! _output =
+          Some (VintN 0)) as O by (apply gss).
+  assert ((PTree.set _output (Vint Int.zero) le) ! _input =
+          Some (Vptr b (Ptrofs.repr ofs))) as I.
+  { rewrite gso. assumption. cbv; congruence. }
+  destruct (Loop O I) as [Exec Out].
+  seq1. 
+  repeat econstructor.
+  seq1. fold f_strlen_loop.
+  eapply Exec.
+  repeat econstructor.
+  eapply Out.
+Qed.
+
+
+(* Test case: On a string of length 2 C light function evaluates to 0 *)
+Lemma strlen_correct_test: forall ge e m b ofs le,
+
+    0 <= ofs < Ptrofs.modulus ->
+    ofs + Z_of_nat 2 < Ptrofs.modulus ->                      
+
+    le!_input = Some (Vptr b (Ptrofs.repr ofs)) ->
+    le!_output = Some (VintZ 0) ->                     
+
+    strlen_mem m b ofs 2%nat ->
+    
+    (* C light expression f_strlen returns O and assigns O to output variable *)
+    exists t le', exec_stmt ge e le m f_strlen.(fn_body) t le' m (Out_return (Some ((VintZ 2),tuint))) /\ (le'!_output) = Some (VintZ 2).
+Proof.
+  intros.
+  inversion_clear H3. inversion_clear H4. inversion_clear H3.
+  repeat eexists.
+  - seq1.
+    -- sset. (* evaluate expression *) repeat econstructor.
+    -- seq1.   
+      * (* loop 1 *)
+        loop. repeat econstructor. repeat gso_assumption. eapply gss. repeat econstructor.
+        rewrite gso. apply gss. cbv. congruence. simpl. ptrofs_to_Z. apply H5. assumption.
+        apply gss.
+        simpl.
+        econstructor.
+        replace (negb (Int.eq c Int.zero)) with true.     
+        econstructor.
+         { replace (Int.eq c Int.zero) with false.
+           auto.
+           rewrite Int.eq_false.
+           reflexivity.
+           assumption. } 
+         rewrite gso. rewrite gso. rewrite gso. apply gss. 1-3: cbv; congruence.
+        repeat econstructor. econstructor. econstructor.
+
+        (* loop 2 *)
+        loop. repeat econstructor. 
+        rewrite gso. rewrite gso. apply gss. 1-2: cbv; congruence. apply gss.
+        repeat econstructor.
+        rewrite gso. apply gss. cbv; congruence.
+        simpl.
+        replace (Ptrofs.unsigned
+                   (Ptrofs.add (Ptrofs.repr ofs) (Ptrofs.mul (Ptrofs.repr 1) (Ptrofs.of_ints (Int.repr 1))))) with (ofs + 1).
+        apply H7.
+        { unfold Ptrofs.of_ints.
+          replace (Int.signed (Int.repr 1)) with 1 by (auto with ints).
+          ptrofs_compute_add_mul. all: nia. }
+ 
+        apply gss.
+        econstructor.
+        replace (negb (Int.eq c0 Int.zero)) with true.      
+        econstructor.
+        { replace (Int.eq c0 Int.zero) with false.
+          auto.
+          rewrite Int.eq_false.
+          reflexivity.
+          assumption. } 
+        rewrite gso. rewrite gso. rewrite gso. apply gss. 1-3: cbv; congruence.
+        repeat econstructor. econstructor. econstructor.
+            
+         (* exit loop *)
+        eapply exec_Sloop_stop1.
+        seq2. seq1. seq1. econstructor. econstructor. rewrite gso. rewrite gso. apply gss. 1-2: cbv; congruence.
+        repeat econstructor.
+        apply gss.
+        repeat econstructor.
+        seq1. repeat econstructor.
+        rewrite gso. apply gss. cbv ; congruence.
+        simpl.
+        replace (Ptrofs.unsigned
+       (Ptrofs.add
+          (Ptrofs.add (Ptrofs.repr ofs)
+             (Ptrofs.mul (Ptrofs.repr 1) (Ptrofs.of_ints (Int.repr 1))))
+          (Ptrofs.mul (Ptrofs.repr 1) (Ptrofs.of_ints (Int.repr 1))))) with (ofs + 1 + 1).
+        apply H4.
+        { unfold Ptrofs.of_ints.
+          replace (Int.signed (Int.repr 1)) with 1 by (auto with ints).
+          ptrofs_compute_add_mul. all: nia. }
+        repeat econstructor.
+        apply gss.
+        econstructor. 
+        replace (negb (Int.eq Int.zero Int.zero)) with false by (auto with ints).
+        econstructor.
+        cbv; congruence.
+        econstructor.
+      * (* return statement *)
+        repeat econstructor.  rewrite gso.  rewrite gso. rewrite gso.  eapply gss. all: cbv; congruence.
+  - rewrite gso.  rewrite gso.  rewrite gso. eapply gss. all: cbv; congruence.
+    Qed.
+
+(* Conditions about the f_strlen loop *)
+
+(* If 0 is read from memory at [b,ofs + len] the output is set to len *)
+Lemma strlen_loop_break_correct:  forall ge e m b ofs outp le,
+      
+      ofs + Z.of_nat outp < Ptrofs.modulus ->
+      0 <= ofs < Ptrofs.modulus ->
+      0 <= Z.of_nat outp < Ptrofs.modulus ->
+
+      (* IF before the loop *s = [b,ofs + outp] and i = outp *)
+      le!_input = Some (Vptr b (Ptrofs.repr (ofs + Z.of_nat outp))) ->
+      le!_output = Some (VintN outp) ->
+      
+      (* and the guard condition is false *)
+      Mem.load Mint8unsigned m b (ofs + (Z_of_nat outp)) = Some (Vint (Int.repr 0)) ->
+
+      (* THEN loop executes to an environment with i = outp [i.e., i stays unchanged] + memory is unchanged *)
+      exists t le', exec_stmt ge e le m f_strlen_loop t le' m Out_normal /\ (le'!_output) = Some (VintN outp).
+Proof.
+  intros.
+  repeat eexists.
+  eapply exec_Sloop_stop1.
+  seq2. seq1. seq1.
+  repeat econstructor.
+  apply H2.
+  repeat econstructor.
+  apply gss.
+  repeat econstructor.
+  seq1.
+  repeat econstructor.
+  rewrite gso. apply gss. cbv ; congruence.
+  simpl.
+  replace (Ptrofs.unsigned (Ptrofs.repr (ofs + Z.of_nat outp))) with (ofs + Z.of_nat outp).
+  apply H4.
+  { ptrofs_compute_add_mul. all: lia. }
+  repeat econstructor.
+  apply gss.
+  econstructor.
+  replace (negb (Int.eq Int.zero Int.zero)) with false by (auto with ints).
+  econstructor.
+  cbv; congruence.
+  econstructor.
+  repeat (rewrite gso). assumption.
+  all: cbv; congruence.
+Qed.
+
+   
+Lemma strlen_loop_body_correct: Archi.ptr64 = false -> forall len ge e m b ofs le,
+      0 <= ofs < Ptrofs.modulus ->
+      Z_of_nat len < Int.modulus ->
+      ofs + Z_of_nat len < Ptrofs.modulus ->
+                       
+      le!_input = Some (Vptr b (Ptrofs.repr (ofs + Z.of_nat len))) ->
+      le!_output = Some (VintN len) ->
+    
+      (exists c, Mem.load chunk m b (ofs + Z.of_nat len) = Some (Vint c) /\c <> Int.zero) ->
+                                         
+      exists t le', exec_stmt ge e le m f_strlen_loop_body t le' m Out_normal /\ le'!_output = Some (VintN (S len)).
+Proof.
+  intros.
+  destruct H5 as [p].
+  repeat eexists.
+  repeat seq1.
+  repeat econstructor. apply H3. repeat econstructor.
+  apply gss.
+  repeat econstructor.
+  repeat econstructor.
+  rewrite gso. apply gss. cbv; congruence.
+  simpl.
+  replace (Ptrofs.unsigned (Ptrofs.repr (ofs + Z.of_nat len))) with (ofs + Z.of_nat len). 
+  apply H5.
+  { ptrofs_compute_add_mul. all: lia. }
+  repeat econstructor.
+  apply gss.
+  econstructor.
+  replace (negb (Int.eq p Int.zero)) with true.
+  repeat econstructor.
+  { replace (Int.eq p Int.zero) with false.
+          auto.
+          rewrite Int.eq_false.
+          reflexivity.
+          apply H5. }
+  repeat econstructor.
+  repeat (rewrite gso).
+  apply H4. 1-3: cbv; congruence.
+  repeat econstructor.
+  unfold VintN.
+  replace (Int.add (Int.repr (Z.of_nat len)) (Int.repr 1)) with (Int.repr (Z.of_nat (S len))). 
+  apply gss.
+  { ints_compute_add_mul.
+    f_equal.
+    lia.
+    split; try lia. cbv; auto.
+    lia. }
+Qed.
                
 
